introduce forall 을 이용해, lemma_for_children 증명 성공 - ...그 다음엔?

src/study/Nemonuri.Study.CSharpSyntaxRewriter2.Modifier/Nemonuri.StratifiedNode.NodeTheory.Common.fst
@@ -132,3 +132,20 @@ let lemma_for_subchildren
   lemma_subchildren_tl_is_subchildren parent subchildren;
   lemma_children_contained_node_level_is_lower_than_parent parent (get_hd subchildren)
 
+let all_nodes_contained_in_children_are_child (#t:eqtype) (#lv:pos) (sn:stratified_node t lv) : prop 
+  = (forall (lv2:pos) (sn2:stratified_node t lv2). (children_contains sn sn2) ==> (is_child sn sn2))
+
+open FStar.Classical.Sugar
+
+let lemma_for_children
+  (#t:eqtype) (#lv:pos) (sn:stratified_node t lv) 
+  : Lemma (ensures (all_nodes_contained_in_children_are_child sn))
+  = introduce forall (lv2:pos) (sn2:stratified_node t lv2{children_contains sn sn2}). ((lv2 < lv) /\ (is_child sn sn2)) with
+    (lemma_children_contained_node_level_is_lower_than_parent sn sn2)
+
+let for_all_children
+  (#t:eqtype) (#lv:pos) (sn:stratified_node t lv)
+  (predicate:stratified_node_predicate t)
+  : Tot (_:bool{all_nodes_contained_in_children_are_child sn})
+  = lemma_for_children sn;
+    for_all sn.children predicate
