src/study/Nemonuri.Study.CSharpSyntaxRewriter2.Modifier/Nemonuri.StratifiedNode.TypeTheory1.fst
@@ -10,16 +10,19 @@ block =
   ;
 
 statement =
-  | argument*
+  | statement_normal: argument*
+  | statement_substituted: substitution_index:nat expression{ this is (not expression_blockless_simple) and (not expression_blockless_substituted) }
   ;
 
 argument =
-  | p0: block block*
-  | p1: blockless_expression
+  | expression
   ;
 
-blockless_expression =
-  | (...)
+expression =
+  | expression_block_containing: blocks:block*{ this.Count >= 1 }
+  | expression_blockless_simple
+  | expression_blockless_complex
+  | expression_blockless_substituted: substitution_index:nat
   ;
 *)
 
@@ -37,21 +40,22 @@ private let lemma_for_all
           (decreases snl)
   = lemma_list_satisfies_for_all_predicate_means_element_satisfies_predicate snl sn predicate; ()
 
-type argument_sum_kind =
-  | Argument_s0
-  | Argument_s1
+type statement_sum_kind =
+  | Statement_normal
+  | Statement_substituted: substitution_index:nat -> statement_sum_kind
 
-type blockless_expression_sum_kind =
-  | Blockless_expression_normal
-  | Blockless_expression_complex
-  | Blockless_expression_substituted: var_index:nat -> blockless_expression_sum_kind
+type expression_sum_kind =
+  | Expression_block_containing
+  | Expression_blockless_simple
+  | Expression_blockless_complex
+  | Expression_blockless_substituted: substitution_index:nat -> expression_sum_kind
 
 type kind =
   | Compilation_unit
   | Block
-  | Statement
-  | Argument: argument_sum_kind -> kind
-  | Blockless_expression: blockless_expression_sum_kind -> kind
+  | Statement: statement_sum_kind -> kind
+  | Argument
+  | Expression: expression_sum_kind -> kind
 
 type data = { 
   kind: kind
@@ -60,18 +64,156 @@ type data = {
 let node (lv:pos) = (stratified_node data lv)
 let node_list (mlv:nat) = (stratified_node_list data mlv)
 
+
 let get_kind (#lv:pos) (sn:node lv)
   : Tot kind
   = sn.value.kind
 
-let is_kind_blockless_expression (#lv:pos) (sn:node lv)
+let get_statement_sum_kind (#lv:pos) (sn:node lv{ Statement? (get_kind sn) })
+  : Tot statement_sum_kind
+  = let Statement v0 = (get_kind sn) in v0
+
+#push-options "--query_stats"
+let rec has_kind_block (#lv:pos) (sn:node lv)
+  : Tot bool (decreases lv)
+  = Block? (get_kind sn) &&
+    (for_all_children sn has_kind_statement)
+
+and has_kind_statement (#lv:pos) (sn:node lv)
+  : Tot bool (decreases lv)
+  = Statement? (get_kind sn) && (
+    match (get_statement_sum_kind sn) with
+    | Statement_normal -> (for_all_children sn has_kind_argument)
+    | Statement_substituted _ -> (get_children_length sn = 1) && (for_all_children sn has_kind_expression)
+    )
+
+and has_kind_argument (#lv:pos) (sn:node lv)
+  : Tot bool (decreases lv)
+  = Argument? (get_kind sn)
+
+and has_kind_expression (#lv:pos) (sn:node lv)
   : Tot bool
-  = (is_leaf sn) && (Blockless_expression? (get_kind sn))
+  = Expression? (get_kind sn)
+#pop-options
 
-let get_blockless_expression_sum_kind (#lv:pos) (sn:node lv{ is_kind_blockless_expression sn })
-  : Tot blockless_expression_sum_kind
-  = let Blockless_expression v0 = (get_kind sn) in v0
+let has_kind_compilation_unit (#lv:pos) (sn:node lv)
+  : Tot bool (decreases lv)
+  = (Compilation_unit? (get_kind sn)) &&
+    (for_all_children sn has_kind_block)
 
+
+
+
+
+
+
+
+let has_kind_statement_normal (#lv:pos) (sn:node lv)
+  : Tot bool
+  = (has_kind_statement sn) && (Statement_normal? (get_statement_sum_kind sn))
+
+let has_kind_statement_substituted (#lv:pos) (sn:node lv)
+  : Tot bool
+  = (has_kind_statement sn) && (Statement_substituted? (get_statement_sum_kind sn))
+
+
+let get_expression_sum_kind (#lv:pos) (sn:node lv{ has_kind_expression sn })
+  : Tot expression_sum_kind
+  = let Expression v0 = (get_kind sn) in v0
+
+let has_kind_expression_block_containing (#lv:pos) (sn:node lv)
+  : Tot bool
+  = (has_kind_expression sn) && (Expression_block_containing? (get_expression_sum_kind sn))
+
+let has_kind_expression_blockless_simple (#lv:pos) (sn:node lv)
+  : Tot bool
+  = (has_kind_expression sn) && (Expression_blockless_simple? (get_expression_sum_kind sn))
+
+let has_kind_expression_blockless_complex (#lv:pos) (sn:node lv)
+  : Tot bool
+  = (has_kind_expression sn) && (Expression_blockless_complex? (get_expression_sum_kind sn))
+
+let has_kind_expression_blockless_substituted (#lv:pos) (sn:node lv)
+  : Tot bool
+  = (has_kind_expression sn) && (Expression_blockless_substituted? (get_expression_sum_kind sn))
+
+
+let get_substitution_index (#lv:pos) (sn:node lv{ (has_kind_statement_substituted sn) || (has_kind_expression_blockless_substituted sn) })
+  : Tot nat
+  = if (has_kind_statement_substituted sn) then
+      Statement_substituted?.substitution_index (get_statement_sum_kind sn) 
+    else
+      Expression_blockless_substituted?.substitution_index (get_expression_sum_kind sn) 
+
+
+let is_valid_expression_block_containing (#lv:pos) (sn:node lv{ has_kind_expression_block_containing sn })
+  : Tot bool
+  = (get_children_length sn >= 1) &&
+    (for_all_children sn has_kind_block)
+
+let is_valid_expression_blockless_simple (#lv:pos) (sn:node lv{ has_kind_expression_blockless_simple sn })
+  : Tot bool
+  = (is_leaf sn)
+
+let is_valid_expression_blockless_complex (#lv:pos) (sn:node lv{ has_kind_expression_blockless_complex sn })
+  : Tot bool
+  = (is_leaf sn)
+
+let is_valid_expression (#lv:pos) (sn:node lv{ has_kind_expression sn })
+  : Tot bool
+  = if (has_kind_expression_block_containing sn) then (is_valid_expression_block_containing sn)
+    else if (has_kind_expression_blockless_simple sn) then (is_valid_expression_blockless_simple sn)
+    else if (has_kind_expression_blockless_complex sn) then (is_valid_expression_blockless_complex sn)
+    else true
+
+let has_kind_expression_and_valid (#lv:pos) (sn:node lv)
+  : Tot bool
+  = (has_kind_expression sn) && (is_valid_expression sn)
+
+let is_valid_argument (#lv:pos) (sn:node lv{ has_kind_argument sn })
+  : Tot bool
+  = (get_children_length sn = 1) &&
+    (has_kind_expression_and_valid (get_child_at sn 0))
+
+let has_kind_argument_and_valid (#lv:pos) (sn:node lv)
+  : Tot bool
+  = (has_kind_argument sn) && (is_valid_argument sn)
+
+let is_valid_statement_normal (#lv:pos) (sn:node lv{ has_kind_statement_normal sn })
+  : Tot bool
+  = (for_all_children sn has_kind_argument_and_valid)
+
+(*
+let rec is_valid_argument_for_statement_substituted (#lv:pos) (sn:node lv{ has_kind_argument_and_valid sn })
+  : Tot bool
+  = 
+*)
+
+(*
+let rec is_valid_expression_for_statement_substituted (#lv:pos) (sn:node lv{ has_kind_expression_and_valid sn })
+  : Tot bool (decreases lv)
+  = if (has_kind_expression_blockless_simple sn) then false
+    else if (has_kind_expression_blockless_substituted sn) then false
+    else if (has_kind_expression_block_containing sn) then (for_all_children sn is_valid_block_for_statement_substituted)
+
+and is_valid_block_for_statement_substituted (#lv:pos) (sn:node lv{ has_kind_block sn })
+  : Tot bool (decreases lv)
+  = (for_all_children sn has_kind_statement) &&
+    (for_all_children sn is_valid_statement_for_statement_substituted)
+
+and is_valid_statement_for_statement_substituted (#lv:pos) (sn:node lv{ has_kind_statement sn })
+  : Tot bool (decreases lv)
+  = if (has_kind_statement_substituted sn) then 
+*)
+
+
+(*
+let is_valid_statement_substituted (#lv:pos) (sn:node lv{ has_kind_statement_substituted sn })
+  : Tot bool
+  = (get_children_length sn = 1) &&
+*)
+
+(*
 let is_kind_blockless_expression_normal (#lv:pos) (sn:node lv)
   : Tot bool
   = (is_kind_blockless_expression sn) && (Blockless_expression_normal? (get_blockless_expression_sum_kind sn))
@@ -129,9 +271,6 @@ private let lemma_test
   (#lv:pos) (sn:node lv{ is_kind_compilation_unit sn && get_children_length sn >= 3 })
   : Lemma (is_kind_block (get_child_at sn 2))
   = ()
-
-(*
-let is_kind_argument_s1 (#lv:pos) (sn:node lv)
-  : Tot bool
-  = (is_branch sn) && (Blockless_expression? sn.value.kind)
 *)
+
+//let is_argument_ready_to_be_substituted
